\subsection{Observed information}

\newcommand{\fpt}{\frac{\partial} {\partial \lambda_{2}}}

\newcommand{\fps}{\frac{\partial^{2}}{\partial\lambda_{1}\partial\lambda_{2}}}


To compute the observed information, again the formulae by \citet{Lys2002} are applied and generalized to the m-variate mixture case. Define the information recursion as follows:
\begin{equation}
%\begin{split}
	\omega_{1}(j_{k};\lambda_{1},\lambda_{2}) = & \, \fps Pr(\vc{O}_{1}, S_{1}=j_{k}) 
	= \fps p_{k} \pi_{j_{k}} b_{j_{k}}(\vc{O}_{1}) 
	\\ =& \fpp \left[ \fpt p_{k} \pi_{j_{k}} b_{j_{k}}(\vc{O}_{1}) \right] 
	\\ =&  \fpp  \bigg\{  \left[ \fpt p_{k} \right]  \pi_{j_{k}} b_{j_{k}}(\vc{O}_{1}) +
		p_{k} \left[ \fpt \pi_{j_{k}} \right]  b_{j_{k}}(\vc{O}_{1}) + 
	\\  &  \, p_{k} \pi_{j_{k}} \left[ \fpt  b_{j_{k}}(\vc{O}_{1}) \right] \bigg\}
	\\  = &  \left[ \fps p_{k} \right] \pi_{j_{k}} b_{j_{k}}(\vc{O}_{1}) + 
	\left[\fpt p_{k} \right] \cdot \left[\fpp \pi_{j_{k}} \right] b_{j_{k}}(\vc{O}_{1}) +
	\\  &    \left[ \fpt p_{k} \right] \pi_{k} \left[ \fpp b_{j_{k}}(\vc{O}_{1}) \right] +
	\left[ \fpp \p_{k} \right] \pi_{j_{k}} b_{j_{k}}(\vc{O}_{1}) + 
	\\ &   \, p_{k} \left[ \fps \pi_{j_{k}} \right] b_{j_{k}}(\vc{O}_{1}) +
	p_{k} \left[ \fpt \pi_{j_{k}} \right] \cdot \left[ \fpp b_{j_{k}}(\vc{O}_{1}) \right] +
	\\ &   \left[ \fpp p_{k} \right] \pi_{j_{k}} \left[ \fpt b_{j_{k}}(\vc{O}_{1}) \right] +
	p_{k} \left[ \fpp \pi_{j_{k}} \right] \cdot \left[ \fpt b_{j_{k}}(\vc{O}_{1}) \right] +
	\\ &   \, p_{k} \pi_{j_{k}} \left[ \fps b_{j_{k}}(\vc{O}_{1}) \right].
%\end{split}
\end{equation}

Similarly, for $t>1$, the information recursion is defined as:
\begin{equation}
%\begin{split}
	\omega_{t}(j_{k};\lambda_{1},\lambda_{2}) =  
	&\frac{\fps Pr(\vc{O}_{1}, \ldots, \vc{O}_{t},S_{t}=j_{k})}{Pr(\vc{O}_{1}, \ldots, \vc{O}_{t-1})}
	\\ = &\sum_{k=1}^{K} \sum_{i=1}^{n_{k}} \Bigg\{ 
	\omega_{t-1}(i;\lambda_{1},\lambda_{2}) a_{ij_{k}} b_{j_{k}}(\vc{O}_{t}) +
	\psi_{t-1}(i;\lambda_{1}) \left[ \fpt a_{ij_{k}} \right] b_{j_{k}}(\vc{O}_{t}) +
	\\  &\psi_{t-1}(i;\lambda_{1})  a_{ij_{k}}  \left[ \fpt b_{j_{k}}(\vc{O}_{t}) \right] +
	\psi_{t-1}(i;\lambda_{2}) \left[ \fpp a_{ij_{k}} \right] b_{j_{k}}(\vc{O}_{t}) + 
	\\ & \psi_{t-1}(i;\lambda_{2}) a_{ij_{k}} \left[ \fpp b_{j_{k}}(\vc{O}_{t})\right]  + 
	\phi_{t-1}(i) \left[ \fps a_{ij_{k}} \right]  b_{j_{k}}(\vc{O}_{t}) +
	\\ & \phi_{t-1}(i) a_{ij_{k}} \left[ \fps b_{j_{k}}(\vc{O}_{t}) \right]  +
	\phi_{t-1}(i) \left[ \fpp a_{ij_{k}} \right] \left[ \fpt b_{j_{k}}(\vc{O}_{t}) \right]  +
	\\ & \phi_{t-1}(i) \left[ \fpt a_{ij_{k}}\right] \left[ \fpp b_{j_{k}}(\vc{O}_{t}) \right]  \Bigg\} 
	\times \frac{1}{\Phi_{t-1}}
%\end{split}
\end{equation}

It is important here to provide the second order partial derivatives of the terms that are involved in the multi-variate case. These are the $b_{j_{k}}(\cdot)$ terms. Remember that these terms can be factored and hence the derivatives can be derived from repeatedly applying the chain rule for products and using equation \ref{partialProd} from above for the first order derivatives: 
\begin{equation}
%\begin{split}
	\fps b_{j_{k}} (\vc{O}_{t}) & = \fps \prod_{i=1}^{m} b_{j_{k}}^{i} (O_{t}^{i}) \\
	& = \fpp \left[ \fpt \prod_{i=1}^{m} b_{j_{k}}^{i} (O_{t}^{i})  \right] \\
	& = \fpp \Bigg\{ \sum_{l=1}^{m} \left[ \prod_{i=1, \ldots, \hat{l}, \ldots, m} b_{j}(O_{t}^{i}) 
	\right] \times \fpt  [b_{j}(O_{t}^{l})] \Bigg\}  \\
	& = \sum_{l=1}^{m} \left[ \fpp \prod_{i=1, \ldots, \hat{l}, \ldots, m} b_{j}(O_{t}^{i}) 
	\right] \times \fpt  \left[b_{j}(O_{t}^{l})]\;+ \\
	&\phantom{=}\;\, \sum_{l=1}^{m}  \left[ \prod_{i=1, \ldots, \hat{l}, \ldots, m} b_{j}(O_{t}^{i}) 
	\right] \times \fpp \fpt  \left[ b_{j}(O_{t}^{l})\right]  \\
	& = \sum_{k=1,k\neq	l}^{m} \sum_{l=1}^{m}  \left[ \prod_{i=1, \ldots, \hat{l}, \hat{k}, \ldots, 
	m} b_{j}(O_{t}^{i}) \right] \fpt  \left[ b_{j}(O_{t}^{k})\right]  \fpt  \left[ b_{j}(O_{t}^{l})\right] \;+ \\
	&\phantom{=}\;\, \sum_{l=1}^{m}  \left[ \prod_{i=1, \ldots, \hat{l}, \ldots, m} b_{j}(O_{t}^{i}) 
	\right] \times \fps  \left[b_{j}(O_{t}^{l}) \right] 
%\end{split}
\end{equation}



 